Mostly reason about case that DescendLessOrEqual finds a snapshot

new/proof/go_etcd_io/etcd/cache/v3.v
@@ -78,8 +78,12 @@ Axiom is_kvItem : loc → kvItem → iProp Σ.
 Axiom less_kvItem : kvItem → kvItem → Prop.
 
 (* for ringbuffer *)
-Definition snap : Type := (w64 * list KeyValue.t).
-Axiom is_snapshotItem : loc → snap → iProp Σ.
+Notation snap := (w64 * list KeyValue.t)%type.
+Definition is_snapshotItem (l : loc) (s : snap) : iProp Σ :=
+  ∃ tree,
+    "#snapshot" ∷ l ↦□ (cache.snapshot.mk s.1 tree) ∗
+    "#tree" ∷ (own_BTree tree is_kvItem less_kvItem (inr <$> s.2) DfracDiscarded).
+
 Definition rev_snapshotItem : snap → w64 := fst.
 
 Axiom is_etcd_kvs :
@@ -115,12 +119,6 @@ Definition own_store (s : loc) (prefix : go_string) : iProp Σ :=
     ) ∗
   "_" ∷ True.
 
-Definition is_snapshot (snap_ptr : loc) (kvs : gmap go_string KeyValue.t) : iProp Σ :=
-  True.
-
-Definition is_etcd_state (rev : w64) (kvs : gmap go_string KeyValue.t) : iProp Σ :=
-  True.
-
 (* FIXME: the history can be empty only if there was a progres notification, but
    no normal watch response. That's the only case in which DescendLessOrEqual
    would never run iter. Otherwise, by the time it's called, DescendLessOrEqual
@@ -132,13 +130,13 @@ Definition is_etcd_state (rev : w64) (kvs : gmap go_string KeyValue.t) : iProp �
 Lemma wp_store__getSnapshot s (rev : w64) prefix :
   {{{ is_pkg_init cache ∗ "Hs" ∷ own_store s prefix }}}
     s @! (go.PointerType cache.store) @! "getSnapshot" #rev
-  {{{ snap_ptr snap_rev err, RET (#snap_ptr, #snap_rev, #err);
+  {{{ snap_ptr (latest_rev : w64) err, RET (#snap_ptr, #latest_rev, #err);
       own_store s prefix ∗
       match err with
       | interface.nil =>
-          (∃ kvs,
-              is_snapshot snap_ptr kvs ∗
-              is_etcd_state snap_rev kvs)
+          (∃ kvs snap_rev,
+              is_snapshotItem snap_ptr (snap_rev, kvs) ∗
+              is_etcd_kvs rev prefix (ordered_kvs_to_map kvs))
       | _ => True
       end
   }}}.
@@ -172,13 +170,39 @@ Proof.
     wp_start as "(@ & %Hlookup & Hitem)".
     wp_auto. wp_alloc rev_ptr2 as "rev2". wp_auto.
     wp_end. iIntros "history_inv". wp_auto. wp_if_destruct.
-    { exfalso. admit. (* TODO: prove is_snapshotItem -> non-null *) }
+    { iExFalso. iNamed "Hitem". iDestruct (typed_pointsto_not_null with "snapshot") as %Hbad.
+      done. }
     iCombineNamed "*_inv" as "Hinv".
     wp_apply (wp_RWMutex__RUnlock with "[$Hrlocked Hinv]").
     { iNamed "Hinv". iFrame "∗#%". }
     iIntros "Hmu". wp_auto.
     iApply "HΨ".
-    iFrame. admit. (* TODO: fill in postcondition *)
+    iFrame.
+    rewrite reverse_lookup_Some in Hlookup. destruct Hlookup as [Hlookup ?].
+    ereplace (?[x] - 1)%nat with (Nat.pred ?x) in Hlookup.
+    2:{ lia. }
+    pose proof (list_elem_of_lookup_2 _ _ _ Hlookup) as Hitemv.
+    rewrite list_elem_of_filter in Hitemv.
+    rewrite -last_lookup in Hlookup.
+    apply last_filter_Some in Hlookup as (old_history & new_history & ? & Hnot).
+    subst. iApply "Hhistory_inv". iPureIntro.
+    split_and!.
+    - instantiate (1:=length old_history).
+      rewrite lookup_app_l; last by len.
+      rewrite lookup_app_r; last by len.
+      rewrite Nat.sub_diag. done.
+    - instantiate (1:=hd (snapshot.(cache.snapshot.rev'), kvs_ordered) new_history).
+      rewrite -app_assoc.
+      rewrite lookup_app_r.
+      2:{ clear. unfold w64. lia. }
+      ereplace (S ?[x] - ?x)%nat with 1%nat by lia.
+      rewrite /= lookup_app /=.
+      destruct new_history; done.
+    - destruct itemv; simpl in *. word.
+    - destruct new_history.
+      + simpl. admit. (* FIXME: handle the case that rev = cache.snapshot.rev *)
+      + simpl. destruct p; simpl in *.
+        rewrite Forall_cons_iff in Hnot. simpl in *. word.
   }
   {
     iIntros "history_inv @". wp_auto.
